CN

STLC/Substitution.lean
@@ -1,3 +1,5 @@
+open Classical
+
 set_option autoImplicit false
 
 inductive Term where
@@ -79,6 +81,7 @@ theorem rename_abs (ρ : Rename) (t : Term) : rename ρ (.abs t) = .abs (rename 
 @[simp]
 theorem rename_app (ρ : Rename) (t₁ t₂ : Term) : rename ρ (.app t₁ t₂) = .app (rename ρ t₁) (rename ρ t₂) := rfl
 
+@[simp]
 theorem rename_id : rename id = id := by
   funext t
   induction t with
@@ -219,6 +222,23 @@ theorem substitutivity {t₁ t₂ : Term} (h : Step t₁ t₂) (σ : Substitutio
     let σ' := ids 0 .: σ >>> rename shift
     exact .step_abs (subst σ' t₁) (subst σ' t₂) (ih σ')
 
+theorem step_rename_of_step {t t' : Term} (ρ : Rename) (step : Step t t') : Step (rename ρ t) (rename ρ t') := by
+  induction step generalizing ρ with
+  | step_beta t u t' eq =>
+    subst t'
+    simp
+    refine .step_beta (rename (up ρ) t) (rename ρ u) (subst (rename ρ u .: ρ >>> ids) t) ?_
+    simp [up]
+  | step_appL t₁ t₂ u step ih =>
+    simp
+    exact .step_appL (rename ρ t₁) (rename ρ t₂) (rename ρ u) (ih ρ)
+  | step_appR t u₁ u₂ step ih =>
+    simp
+    exact .step_appR (rename ρ t) (rename ρ u₁) (rename ρ u₂) (ih ρ)
+  | step_abs t₁ t₂ step ih =>
+    simp
+    exact .step_abs (rename (up ρ) t₁) (rename (up ρ) t₂) (ih (up ρ))
+
 inductive Ty where
   | base
   | arrow (a b : Ty)
@@ -242,9 +262,16 @@ theorem agrees_up_iff {α : Type} {Γ Δ : Nat → α} {ρ : Rename} (A B : α) 
   simp [up, agrees]
 
 @[simp]
+theorem agrees_id {α : Type} {Γ : Nat → α} : Γ ⤳[id] Γ := rfl
+
+@[simp]
 theorem agrees_shift {α : Type} {Γ : Nat → α} {A : α} : Γ ⤳[shift] (A .: Γ) := by
   funext x
   simp
+
+@[simp]
+theorem agrees_comp {α : Type} {Γ₁ Γ₂ Γ₃ : Nat → α} (ρ₁ ρ₂ : Rename) (ag₁ : Γ₁ ⤳[ρ₁] Γ₂) (ag₂ : Γ₂ ⤳[ρ₂] Γ₃) : Γ₁ ⤳[ρ₁ >>> ρ₂] Γ₃ := by
+  simp_all [agrees]
 
 inductive HasType : TyCtx → Term → Ty → Prop where
   | type_var (Γ : TyCtx) (x : Nat) (A : Ty) : Γ x = A → HasType Γ (.var x) A
@@ -312,3 +339,266 @@ theorem preservation_steps {Γ : TyCtx} {t t' : Term} {A : Ty} (steps : Steps t 
   induction steps with
   | refl => exact ty
   | next t₁ t₂ t₃ step rest ih => exact ih (preservation step ty)
+
+theorem rename_abs_inv {t u : Term} {ρ : Rename} (eq : rename ρ t = .abs u) : ∃ t', t = .abs t' ∧ rename (up ρ) t' = u := by
+  cases t with
+  | var | app => simp at eq
+  | abs t' =>
+    simp at eq
+    exact ⟨t', rfl, eq⟩
+
+theorem rename_step_of_step_rename {t₁ t₂ : Term} {ρ : Rename} (step : Step (rename ρ t₁) t₂) : ∃ t₂', rename ρ t₂' = t₂ ∧ Step t₁ t₂' := by
+  induction t₁ generalizing ρ t₂ with
+  | var x =>
+    simp at step
+    nomatch step
+  | abs t₁ ih =>
+    simp at step
+    cases step with
+    | step_abs _ t₂ step =>
+      have ⟨t₂', eq, step'⟩ := ih step
+      exact ⟨.abs t₂', by simp [eq], .step_abs _ _ step'⟩
+  | app t₁ u ih₁ ih₂ =>
+    simp at step
+    generalize h : rename ρ t₁ = t₁' at step
+    cases step with
+    | step_beta s _ _ eq =>
+      subst t₂
+      have ⟨t₁', eq', rename_eq⟩ := rename_abs_inv h
+      subst t₁ s
+      exact ⟨subst (u .: ids) t₁', by simp [up], .step_beta t₁' u _ rfl⟩
+    | step_appL t₁' t₂ _ step =>
+      subst t₁'
+      have ⟨t₂', eq, step'⟩ := ih₁ step
+      subst t₂
+      exact ⟨.app t₂' u, by simp, .step_appL _ _ _ step'⟩
+    | step_appR t₁ u u' step =>
+      subst t₁'
+      have ⟨u'', eq, step'⟩ := ih₂ step
+      subst u'
+      exact ⟨.app t₁ u'', by simp, .step_appR _ _ _ step'⟩
+
+mutual
+
+inductive Neutral : Term → Prop where
+  | ne_var (x : Nat) : Neutral (.var x)
+  | ne_app (t u : Term) : Neutral t → Normal u → Neutral (.app t u)
+
+inductive Normal : Term → Prop where
+  | no_ne (t : Term) : Neutral t → Normal t
+  | no_abs (t : Term) : Normal t → Normal (.abs t)
+
+end
+
+mutual
+
+theorem no_step_of_neutral {t t' : Term} (ne : Neutral t) (step : Step t t') : False := by
+  cases ne with
+  | ne_var x => nomatch step
+  | ne_app t u ne no =>
+    cases step with
+    | step_beta t _ _ eq => nomatch ne
+    | step_appL _ t' _ step => exact no_step_of_neutral ne step
+    | step_appR _ _ u' step => exact no_step_of_normal no step
+
+theorem no_step_of_normal {t t' : Term} (no : Normal t) (step : Step t t') : False := by
+  cases no with
+  | no_ne t ne => exact no_step_of_neutral ne step
+  | no_abs t no =>
+    cases step with
+    | step_abs _ t' step => exact no_step_of_normal no step
+
+end
+
+def Term.isAbs : Term → Bool
+  | .abs _ => true
+  | .var _ | .app _ _ => false
+
+@[simp]
+theorem isAbs_abs {t : Term} : (Term.abs t).isAbs = true := rfl
+
+@[simp]
+theorem isAbs_var {x : Nat} : (Term.var x).isAbs = false := rfl
+
+@[simp]
+theorem isAbs_app {t₁ t₂ : Term} : (Term.app t₁ t₂).isAbs = false := rfl
+
+theorem normal_or_neutral_of_no_step {t : Term} (step : ∀ t', ¬Step t t') : if t.isAbs then Normal t else Neutral t := by
+  induction t with
+  | var x =>
+    simp
+    exact .ne_var x
+  | abs t ih =>
+    simp
+    have h (t' : Term) (step' : Step t t') : False := step (.abs t') (.step_abs t t' step')
+    have no : Normal t := by
+      have := ih h
+      split at this
+      next => exact this
+      next => exact .no_ne _ this
+    exact .no_abs t no
+  | app t₁ t₂ ih₁ ih₂ =>
+    simp
+    refine .ne_app t₁ t₂ ?_ ?_
+    . if step' : ∃ t₁', Step t₁ t₁' then
+        have ⟨t₁', step'⟩ := step'
+        exact False.elim (step (.app t₁' t₂) (.step_appL t₁ t₁' t₂ step'))
+      else
+        simp at step'
+        have ih₁ := ih₁ step'
+        match t₁ with
+        | .abs t₁ => exact False.elim (step _ (.step_beta t₁ t₂ _ rfl))
+        | .var _ | .app _ _ => exact ih₁
+    . if step' : ∃ t₂', Step t₂ t₂' then
+        have ⟨t₂', step'⟩ := step'
+        exact False.elim (step (.app t₁ t₂') (.step_appR t₁ t₂ t₂' step'))
+      else
+        simp at step'
+        have ih₂ := ih₂ step'
+        split at ih₂
+        next => exact ih₂
+        next => exact .no_ne _ ih₂
+
+theorem progress {Γ : TyCtx} {t : Term} {A : Ty} (ty : HasType Γ t A) : Normal t ∨ ∃ t', Step t t' := by
+  induction ty with
+  | type_var Γ x A h => exact .inl (.no_ne (.var x) (.ne_var x))
+  | type_abs Γ t A B ty ih =>
+    match ih with
+    | .inl no => exact .inl (.no_abs t no)
+    | .inr ⟨t', step⟩ => exact .inr ⟨.abs t', .step_abs t t' step⟩
+  | type_app Γ t u A B tyt tyu iht ihu =>
+    match iht with
+    | .inl no₁ =>
+      match ihu with
+      | .inl no₂ =>
+        cases no₁ with
+        | no_ne t ne => .exact .inl (.no_ne (.app t u) (.ne_app t u ne no₂))
+        | no_abs t no₁ => exact .inr ⟨subst (u .: ids) t, .step_beta t u _ rfl⟩
+      | .inr ⟨u', step⟩ => exact .inr ⟨.app t u', .step_appR t u u' step⟩
+    | .inr ⟨t', step⟩ => exact .inr ⟨.app t' u, .step_appL t t' u step⟩
+
+inductive SN : Term → Prop where
+  | intro (t : Term) (ih : ∀ t', Step t t' → SN t') : SN t
+
+theorem SN_step {t t' : Term} (step : Step t t') (sn : SN t) : SN t' := by
+  cases sn with
+  | intro _ h => exact h t' step
+
+theorem SN_steps {t t' : Term} (steps : Steps t t') (sn : SN t) : SN t' := by
+  induction steps with
+  | refl => exact sn
+  | next t₁ t₂ t₃ step rest ih => exact ih (SN_step step sn)
+
+theorem SN_of_SN_app {t u : Term} (sn : SN (.app t u)) : SN t ∧ SN u := by
+  generalize h : Term.app t u = s at sn
+  induction sn generalizing t u with
+  | intro t'' _ ih =>
+    subst t''
+    refine ⟨.intro t fun t' step => ?_, .intro u fun u' step => ?_⟩
+    . exact (ih (.app t' u) (.step_appL t t' u step) rfl).1
+    . exact (ih (.app t u') (.step_appR t u u' step) rfl).2
+
+theorem SN_of_SN_rename {t : Term} {ρ : Rename} (sn : SN (rename ρ t)) : SN t := by
+  generalize h : rename ρ t = s at sn
+  induction sn generalizing t ρ with
+  | intro t' h ih =>
+    subst t'
+    refine .intro t (fun t' step => ?_)
+    exact ih (rename ρ t') (step_rename_of_step ρ step) rfl
+
+theorem SN_rename_of_SN {t : Term} {ρ : Rename} (sn : SN t) : SN (rename ρ t) := by
+  induction sn with
+  | intro t h ih =>
+    refine .intro (rename ρ t) (fun t' step => ?_)
+    have ⟨t'', eq, step'⟩ := rename_step_of_step_rename step
+    subst t'
+    exact ih t'' step'
+
+def Red (Γ : TyCtx) (t : Term) (A : Ty) : Prop :=
+  match A with
+  | .base => HasType Γ t .base ∧ SN t
+  | .arrow A B => HasType Γ t (.arrow A B) ∧ ∀ ρ Δ u, Γ ⤳[ρ] Δ → Red Δ u A → Red Δ (.app (rename ρ t) u) B
+
+theorem HasType_of_Red {Γ : TyCtx} {t : Term} {A : Ty} (red : Red Γ t A) : HasType Γ t A := by
+  cases A with
+  | base => simp_all [Red]
+  | arrow A B => simp_all [Red]
+
+theorem Red_step {Γ : TyCtx} {t t' : Term} {A : Ty} (red : Red Γ t A) (step : Step t t') : Red Γ t' A := by
+  induction A generalizing Γ t t' with
+  | base =>
+    simp [Red] at *
+    exact ⟨preservation step red.1, SN_step step red.2⟩
+  | arrow A B ih₁ ih₂ =>
+    simp [Red] at *
+    refine ⟨preservation step red.1, ?_⟩
+    intro ρ Δ u ag red'
+    have red'' := red.2 ρ Δ u ag red'
+    exact ih₂ red'' (.step_appL (rename ρ t) (rename ρ t') u (step_rename_of_step ρ step))
+
+theorem CN₂ {Γ : TyCtx} {t t' : Term} {A : Ty} (red : Red Γ t A) (steps : Steps t t') : Red Γ t' A := by
+  induction steps with
+  | refl => exact red
+  | next t₁ t₂ t₃ step rest ih => exact ih (Red_step red step)
+
+theorem CN₁₃ {Γ : TyCtx} {t : Term} {A : Ty} : (Red Γ t A → SN t) ∧ (HasType Γ t A → ¬t.isAbs → (∀ t', Step t t' → Red Γ t' A) → Red Γ t A) := by
+  induction A generalizing Γ t with
+  | base =>
+    refine ⟨?_, ?_⟩
+    . simp [Red]
+    . intro ty ne cls
+      simp [Red, ty]
+      simp [Red] at cls
+      exact .intro t (fun t' step => (cls t' step).2)
+  | arrow A B ihA ihB =>
+    refine ⟨?_, ?_⟩
+    . simp [Red]
+      intro ty arg
+      have (t' : Term) : ¬Step (.var 0) t' := no_step_of_neutral (t' := t') (.ne_var 0)
+      have : Red (A .: Γ) (.var 0) A := ihA.2 (.type_var _ _ _ rfl) (by simp) (by simp [this])
+      have : Red (A .: Γ) ((rename shift t).app (.var 0)) B := arg shift (A .: Γ) (.var 0) (by simp) this
+      have : SN ((rename shift t).app (.var 0)) := ihB.1 this
+      exact SN_of_SN_rename (SN_of_SN_app this).1
+    . intro ty ne cls
+      refine ⟨ty, fun ρ Δ u ag red => ?_⟩
+      have snu : SN u := ihA.1 red
+
+      induction snu with
+      | intro u h ih =>
+        refine ihB.2 ?_ (by simp) ?_
+        . have : HasType Δ (rename ρ t) (.arrow A B) := HasType_rename ty ag
+          exact .type_app Δ (rename ρ t) u A B this (HasType_of_Red red)
+        . intro t' step
+          generalize h : rename ρ t = ρt at step
+          cases step with
+          | step_beta ρt u u' eq =>
+            match t with
+            | .abs t => simp at ne
+            | .var _ | .app _ _ => simp at h
+          | step_appL ρt ρt' u step =>
+            subst ρt
+            have ⟨t', eq, step'⟩ := rename_step_of_step_rename step
+            subst ρt'
+            have red' : Red Γ t' (.arrow A B) := cls t' step'
+            simp [Red] at red'
+            exact red'.2 ρ Δ u ag red
+          | step_appR ρt u u' step =>
+            subst ρt
+            exact ih u' step (Red_step red step)
+
+theorem CN₁ {Γ : TyCtx} {t : Term} {A : Ty} (red : Red Γ t A) : SN t := CN₁₃.1 red
+
+-- This "Neutrality" comes from Girard's "Proofs and Types" and is different from the Neutral above.
+theorem CN₃ {Γ : TyCtx} {t : Term} {A : Ty} (ty : HasType Γ t A) (ne : ¬t.isAbs) (cls : ∀ t', Step t t' → Red Γ t' A) : Red Γ t A :=
+  CN₁₃.2 ty ne cls
+
+theorem red_rename_of_red_ag {Γ Δ : TyCtx} {t : Term} {A : Ty} {ρ : Rename} (red : Red Γ t A) (ag : Γ ⤳[ρ] Δ) : Red Δ (rename ρ t) A := by
+  induction A generalizing Γ Δ t ρ with
+  | base =>
+    simp [Red] at *
+    exact ⟨HasType_rename red.1 ag, SN_rename_of_SN red.2⟩
+  | arrow A B ihA ihB =>
+    simp [Red] at *
+    refine ⟨HasType_rename red.1 ag, ?_⟩
+    intro ρ' Δ' u ag' red'
+    exact red.2 (ρ >>> ρ') Δ' u (agrees_comp ρ ρ' ag ag') red'
